coq/Derives.v
@@ -1,6 +1,6 @@
 (** * Derivability *)
 
-Require Import List Alg.
+Require Import List ListSet Bool Lia Alg SemTactics.
 
 (** [derives pub t] when [t] can be derived using the terms in [pub]. *)
 
@@ -17,4 +17,205 @@ Inductive derives (pub: list alg): alg -> Prop :=
 | Der_scnd: forall x y, derives pub (Pr x y) -> derives pub y
 | Der_decr: forall x y,
     derives pub (En x y) -> derives pub (inv y) -> derives pub x.
-Hint Resolve Der_tagg Der_pair Der_encr Der_hash : core.
+Hint Constructors derives : core.
+
+(* There is no way to implement derives directly in code.  There is an
+   easy way to do it with analyze-then-synthesize.  Here is the
+   algorithm used in CPSA and in the role compiler:
+
+synth(T, t): bool :=
+  if t in T return true;
+  if t = (t1, t2) return synth t1 && synth t2;
+  if t = (enc t1 t2) return synth t1 && synth t2;
+  if t = (hash t1) return synth t1;
+  if t = "..." return true.
+
+analyze(T): set of terms :=
+  while T changes do
+      let t = some element in T;
+      if t = (t1, t2) then add t1 and t2 to T
+      else if t = (enc t1 t2) and synth(T, invk(t2)) then add t1 to T;
+   done;
+   return T.
+*)
+
+(* synth pub t when t can be synthesized using the terms in pub. *)
+Inductive synth (pub: alg -> Prop): alg -> Prop :=
+| Synth_mem: forall x: alg, pub x -> synth pub x
+| Synth_tag: forall i, synth pub (Tg i)
+| Synth_pair: forall x y,
+    synth pub x -> synth pub y -> synth pub (Pr x y)
+| Synth_encr: forall x y,
+    synth pub x -> synth pub y -> synth pub (En x y)
+| Synth_hash: forall x,
+    synth pub x -> synth pub (Hs x).
+Hint Constructors synth : core.
+
+(* analyze pub t when t can be analyzed using the terms in pub. *)
+Inductive analyze (pub: list alg): alg -> Prop :=
+| Analyze_mem: forall x: alg, In x pub -> analyze pub x
+| Analyze_frst: forall x y, analyze pub (Pr x y) -> analyze pub x
+| Analyze_scnd: forall x y, analyze pub (Pr x y) -> analyze pub y
+| Analyze_decr: forall x y,
+    analyze pub (En x y) -> synth (analyze pub) (inv y) -> analyze pub x.
+
+Theorem derives_implies_analyze_then_synth:
+  forall pub x, derives pub x -> synth (analyze pub) x.
+Proof.
+  intros pub x H.
+  induction H; auto.
+  - apply Synth_mem; apply Analyze_mem; assumption.
+  - inv IHderives; auto.
+    apply Analyze_frst in H0.
+    apply Synth_mem; assumption.
+  - inv IHderives; auto.
+    apply Analyze_scnd in H0.
+    apply Synth_mem; assumption.
+  - inv IHderives1; auto.
+    apply Analyze_decr in H1; auto.
+Qed.
+
+(* Failed attempt that the final Theorem *)
+
+Theorem analyze_then_synth_implies_derives:
+  forall pub x, synth (analyze pub) x -> derives pub x.
+Proof.
+  intros pub x H.
+  induction H; auto.
+  induction H.
+  - apply Der_mem; auto.
+  - eapply Der_frst; eauto.
+  - eapply Der_scnd; eauto.
+  - eapply Der_decr; eauto.
+    clear IHanalyze H x.
+    (* HELP!!! *)
+    give_up.
+Abort.
+
+(* Analyze stratified *)
+
+Inductive analyze_strat (pub: list alg): nat -> alg -> Prop :=
+| Analyze_strat_mem: forall x,
+    In x pub ->
+    analyze_strat pub 0 x
+| Analyze_strat_incl: forall n x,
+    analyze_strat pub n x ->
+    analyze_strat pub (S n) x
+| Analyze_strat_frst: forall n x y,
+    analyze_strat pub n (Pr x y) ->
+    analyze_strat pub (S n) x
+| Analyze_strat_scnd: forall n x y,
+    analyze_strat pub n (Pr x y) ->
+    analyze_strat pub (S n) y
+| Analyze_strat_decr: forall n x y,
+    analyze_strat pub n (En x y) ->
+    synth (analyze_strat pub n) (inv y) ->
+    analyze_strat pub (S n) x.
+Hint Constructors analyze_strat : core.
+
+Lemma analyze_strat_zero:
+  forall pub t,
+    analyze_strat pub 0 t <-> In t pub.
+Proof.
+  split; intros.
+  - inv H; auto.
+  - apply Analyze_strat_mem; auto.
+Qed.
+
+Lemma analyze_strat_zero_then_synth:
+  forall pub t,
+    synth (analyze_strat pub 0) t <-> synth (fun y => In y pub) t.
+Proof.
+  split; intros.
+  - induction H; simpl; auto.
+    rewrite analyze_strat_zero in H.
+    apply Synth_mem; auto.
+  - induction H; simpl; auto.
+Qed.
+
+Lemma synth_implies_derives:
+  forall pub x, synth (fun y => In y pub) x -> derives pub x.
+Proof.
+  intros pub x H.
+  induction H; auto.
+Qed.
+
+Lemma analyze_strat_derives:
+  forall pub n t,
+    synth (analyze_strat pub n) t -> derives pub t.
+Proof.
+  induction n; intros.
+  - rewrite analyze_strat_zero_then_synth in H.
+    apply synth_implies_derives; auto.
+  - induction H; simpl; auto.
+    inv H.
+    + apply IHn.
+      apply Synth_mem; auto.
+    + apply Der_frst with (y := y); auto.
+    + apply Der_scnd with (x := x0); auto.
+    + apply IHn in H2.
+      apply Der_decr with (y := y); auto.
+Qed.
+
+Lemma analyze_strat_monotonic_1:
+  forall pub m t,
+    synth (analyze_strat pub m) t ->
+    synth (analyze_strat pub (S m)) t.
+Proof.
+  intros.
+  induction H; simpl; auto.
+Qed.
+
+Lemma analyze_strat_monotonic_2:
+  forall pub m n t,
+    synth (analyze_strat pub m) t ->
+    synth (analyze_strat pub (n + m)) t.
+Proof.
+  intros.
+  induction n; simpl; auto.
+  apply analyze_strat_monotonic_1; auto.
+Qed.
+
+Lemma analyze_strat_monotonic:
+  forall pub m n t,
+    m <= n ->
+    synth (analyze_strat pub m) t ->
+    synth (analyze_strat pub n) t.
+Proof.
+  intros pub m n t H G.
+  apply analyze_strat_monotonic_2 with (n := n - m) in G.
+  assert (F: n - m + m = n).
+  - lia.
+  - rewrite F in G; auto.
+Qed.
+
+(* Reflection for synth *)
+
+Fixpoint synthb (pub: list alg) t: bool :=
+  set_mem alg_dec t pub ||
+          match t with
+          | Pr x y => synthb pub x && synthb pub y
+          | En x y => synthb pub x && synthb pub y
+          | Hs x => synthb pub x
+          | Tg _ => true
+          | _ => false
+          end.
+
+Lemma synthb_correct :
+  forall pub x, synth (fun y => In y pub) x <-> synthb pub x = true.
+Proof.
+  split.
+  - intro H.
+    induction H; try apply orb_true_iff; intuition.
+    destruct x; apply orb_true_iff; left; apply set_mem_correct2; auto.
+  - induction x; intro H; simpl in H; apply orb_true_iff in H;
+      destruct H; auto;
+        try match goal with
+            | [ H: set_mem alg_dec _ pub = true |- _ ] =>
+              apply set_mem_correct1 in H; auto
+            end; try intuition.
+    + apply andb_true_iff in H.
+      destruct H; auto.
+    + apply andb_true_iff in H.
+      destruct H; auto.
+Qed.
